secure_api/merkle_tree/MerkleTree.New.Low.fst
@@ -332,7 +332,8 @@ val hash_2:
      S.equal (Rgl?.r_repr hreg h1 dst)
        (High.hash_2
          (Rgl?.r_repr hreg h0 src1)
-         (Rgl?.r_repr hreg h0 src2))))
+         (Rgl?.r_repr hreg h0 src2))
+         ))
 #reset-options "--z3rlimit 40 --max_fuel 0"
 let hash_2 src1 src2 dst =
   let hh0 = HST.get () in
@@ -422,14 +423,14 @@ inline_for_extraction let merkle_tree_size_lg = 32ul
 // `hs`: a 2-dim store for hashes, where `hs[0]` contains leaf hash values.
 // `rhs_ok`: to check the rightmost hashes are up-to-date
 // `rhs`: a store for "rightmost" hashes, manipulated only when required to
-//        calculate some merkle parhs that need the rightmost hashes
+//        calculate some merkle paths that need the rightmost hashes
 //        as a part of them.
 // `mroot`: during the construction of `rhs` we can also calculate the Merkle
 //          root of the tree. If `rhs_ok` is true then it has the up-to-date
 //          root value.
 noeq type merkle_tree =
 | MT: offset:offset_t ->
-      i:index_t -> j:index_t{j >= i /\ add64_fits offset j} ->
+      i:index_t -> j:index_t{i <= j /\ add64_fits offset j} ->
       hs:hash_vv{V.size_of hs = merkle_tree_size_lg} ->
       rhs_ok:bool ->
       rhs:hash_vec{V.size_of rhs = merkle_tree_size_lg} ->
@@ -2593,6 +2594,298 @@ let mt_flush mt =
   assert (UInt.fits (U64.v off + U32.v j1) 64);
   let jo = join_offset off j1 in
   mt_flush_to mt jo
+#reset-options
+
+
+/// Retraction
+
+#reset-options "--z3rlimit 50 --initial_fuel 1 --max_fuel 1 --initial_ifuel 0 --max_ifuel 0"
+private val mt_retract_to_:
+  hs:hash_vv{V.size_of hs = merkle_tree_size_lg} ->
+  lv:uint32_t{lv < V.size_of hs} ->
+  i:index_t ->
+  s:index_t ->
+  j:index_t{i <= s && s <= j && U32.v j < pow2 (U32.v (V.size_of hs) - U32.v lv)} 
+-> HST.ST unit
+   (requires (fun h0 ->
+     RV.rv_inv h0 hs /\
+     mt_safe_elts h0 lv hs i j))
+   (ensures (fun h0 _ h1 -> 
+     // memory safety
+     (modifies (loc_union
+                 (RV.rv_loc_elems h0 hs lv (V.size_of hs))
+                 (V.loc_vector_within hs lv (V.size_of hs)))
+              h0 h1) /\
+     RV.rv_inv h1 hs /\
+     mt_safe_elts h1 lv hs i s /\
+     // correctness
+     (mt_safe_elts_spec h0 lv hs i j;
+     S.equal (RV.as_seq h1 hs)
+             (High.mt_retract_to_
+               (RV.as_seq h0 hs) (U32.v lv)
+               (U32.v i) (U32.v s) (U32.v j)))
+     ))
+   (decreases (U32.v merkle_tree_size_lg - U32.v lv))
+
+#reset-options "--z3rlimit 800 --max_fuel 1 --admit_smt_queries true"
+private let rec mt_retract_to_ hs lv i s j =
+  let hh0 = HST.get () in
+
+  // Base conditions
+  mt_safe_elts_rec hh0 lv hs i j;
+  V.loc_vector_within_included hs 0ul lv;
+  V.loc_vector_within_included hs lv (lv + 1ul);
+  V.loc_vector_within_included hs (lv + 1ul) (V.size_of hs);
+  V.loc_vector_within_disjoint hs lv (lv + 1ul) (lv + 1ul) (V.size_of hs);
+
+  if lv >= V.size_of hs then ()
+  else begin
+
+    // 1) Retract hashes at level `lv`.
+    let hvec = V.index hs lv in
+    let old_len = j - offset_of i in
+    let new_len = s - offset_of i in
+    let retracted = RV.shrink hvec new_len in  
+
+    let hh1 = HST.get () in
+
+    // 1-0) Basic disjointness conditions for `RV.assign`
+    V.forall2_forall_left hh0 hs 0ul (V.size_of hs) lv
+      (fun b1 b2 -> HH.disjoint (Rgl?.region_of hvreg b1)
+                                (Rgl?.region_of hvreg b2));
+    V.forall2_forall_right hh0 hs 0ul (V.size_of hs) lv
+      (fun b1 b2 -> HH.disjoint (Rgl?.region_of hvreg b1)
+                                (Rgl?.region_of hvreg b2));
+    V.forall_preserved
+      hs 0ul lv
+      (fun b -> HH.disjoint (Rgl?.region_of hvreg hvec)
+                            (Rgl?.region_of hvreg b))
+      (RV.loc_rvector hvec)
+      hh0 hh1;
+    V.forall_preserved
+      hs (lv + 1ul) (V.size_of hs)
+      (fun b -> HH.disjoint (Rgl?.region_of hvreg hvec)
+                            (Rgl?.region_of hvreg b))
+      (RV.loc_rvector hvec)
+      hh0 hh1;
+    assert (Rgl?.region_of hvreg hvec == Rgl?.region_of hvreg retracted);
+
+    // 1-1) For the `modifies` postcondition.
+    assert (modifies (RV.rs_loc_elem hvreg (V.as_seq hh0 hs) (U32.v lv)) hh0 hh1);
+
+    // 1-2) Preservation
+    RV.rv_loc_elems_preserved
+      hs (lv + 1ul) (V.size_of hs)
+      (RV.loc_rvector (V.get hh0 hs lv)) hh0 hh1;
+
+    // 1-3) For `mt_safe_elts`
+    assert (V.size_of retracted == new_len);
+    mt_safe_elts_preserved
+      (lv + 1ul) hs (i / 2ul) (j / 2ul)
+      (RV.loc_rvector (V.get hh0 hs lv)) hh0 hh1;
+
+    // 1-4) For the `rv_inv` postcondition
+    RV.rs_loc_elems_elem_disj
+      hvreg (V.as_seq hh0 hs) (V.frameOf hs)
+      0 (U32.v (V.size_of hs)) 0 (U32.v lv) (U32.v lv);
+    RV.rs_loc_elems_parent_disj
+      hvreg (V.as_seq hh0 hs) (V.frameOf hs)
+      0 (U32.v lv);
+    RV.rv_elems_inv_preserved
+      hs 0ul lv (RV.loc_rvector (V.get hh0 hs lv))
+      hh0 hh1;
+    assert (RV.rv_elems_inv hh1 hs 0ul lv);
+    RV.rs_loc_elems_elem_disj
+      hvreg (V.as_seq hh0 hs) (V.frameOf hs)
+      0 (U32.v (V.size_of hs))
+      (U32.v lv + 1) (U32.v (V.size_of hs))
+      (U32.v lv);
+    RV.rs_loc_elems_parent_disj
+      hvreg (V.as_seq hh0 hs) (V.frameOf hs)
+      (U32.v lv + 1) (U32.v (V.size_of hs));
+    RV.rv_elems_inv_preserved
+      hs (lv + 1ul) (V.size_of hs) (RV.loc_rvector (V.get hh0 hs lv))
+      hh0 hh1;
+    assert (RV.rv_elems_inv hh1 hs (lv + 1ul) (V.size_of hs));
+
+    assert (rv_itself_inv hh1 hs);
+    assert (elems_reg hh1 hs);
+
+    // 1-5) Correctness
+    assert (S.equal (RV.as_seq hh1 retracted)
+                    (S.slice (RV.as_seq hh0 (V.get hh0 hs lv)) 0 (U32.v new_len)));
+
+    RV.assign hs lv retracted;  
+    
+    let hh2 = HST.get() in       
+
+    // 2-1) For the `modifies` postcondition.
+    assert (modifies (V.loc_vector_within hs lv (lv + 1ul)) hh1 hh2);
+    assert (modifies (loc_union
+                       (RV.rs_loc_elem hvreg (V.as_seq hh0 hs) (U32.v lv))
+                       (V.loc_vector_within hs lv (lv + 1ul))) hh0 hh2);
+
+    // 2-2) Preservation
+    V.loc_vector_within_disjoint hs lv (lv + 1ul) (lv + 1ul) (V.size_of hs);
+    RV.rv_loc_elems_preserved
+      hs (lv + 1ul) (V.size_of hs)
+      (V.loc_vector_within hs lv (lv + 1ul)) hh1 hh2;
+
+    // 2-3) For `mt_safe_elts`
+    assert (V.size_of (V.get hh2 hs lv) == s - offset_of i);
+    mt_safe_elts_preserved
+      (lv + 1ul) hs (i / 2ul) (j / 2ul)
+      (V.loc_vector_within hs lv (lv + 1ul)) hh1 hh2;
+
+    // 2-4) Correctness
+    RV.as_seq_sub_preserved hs 0ul lv (loc_rvector retracted) hh0 hh1;
+    RV.as_seq_sub_preserved hs (lv + 1ul) merkle_tree_size_lg (loc_rvector retracted) hh0 hh1;
+    assert (S.equal (RV.as_seq hh2 hs)
+                    (S.append
+                      (RV.as_seq_sub hh0 hs 0ul lv)
+                      (S.cons (RV.as_seq hh1 retracted)
+                              (RV.as_seq_sub hh0 hs (lv + 1ul) merkle_tree_size_lg))));
+    as_seq_sub_upd hh0 hs lv (RV.as_seq hh1 retracted);
+
+    // if `lv = 31` then `i <= s <= j < 2` thus `os = oi`,
+    // contradicting the branch.
+    // assert (lv + 1ul < merkle_tree_size_lg);
+    // assert (U32.v (j / 2ul) < pow2 (32 - U32.v (lv + 1ul)));
+    // assert (RV.rv_inv hh2 hs);
+    // assert (mt_safe_elts hh2 (lv + 1ul) hs (i / 2ul) (j / 2ul));
+    
+    assert (S.equal (S.slice (V.as_seq hh0 hvec) 0 (U32.v new_len)) 
+                    (S.slice (V.as_seq hh1 retracted) 0 (U32.v new_len)));
+    assert (S.equal (S.slice (RV.as_seq hh1 hs) 0 (U32.v lv))
+                    (S.slice (RV.as_seq hh2 hs) 0 (U32.v lv)));
+    if lv + 1ul >= V.size_of hs then () else
+    begin
+      assert (RV.rv_inv hh2 hs);
+      assume (mt_safe_elts hh2 lv hs i j);
+      assume (mt_safe_elts hh2 lv hs (i/2ul) (j/2ul));
+      assume (mt_safe_elts hh2 lv hs (i/2ul) (s/2ul));
+      mt_retract_to_ hs (lv + 1ul) (i / 2ul) (s / 2ul) (j / 2ul)
+    end;
+    let hh_end = HST.get () in
+    admit()
+  end
+ 
+    // /// 3) Recursion
+    // mt_retract_to_ (lv + 1ul) hs (pi / 2ul) (i / 2ul)
+    //   (Ghost.hide ( j / 2ul));
+    // let hh3 = HST.get () in
+
+    // // 3-0) Memory safety brought from the postcondition of the recursion
+    // assert (modifies
+    //          (loc_union
+    //            (loc_union
+    //              (RV.rs_loc_elem hvreg (V.as_seq hh0 hs) (U32.v lv))
+    //              (V.loc_vector_within hs lv (lv + 1ul)))
+    //            (loc_union
+    //              (RV.rv_loc_elems hh0 hs (lv + 1ul) (V.size_of hs))
+    //              (V.loc_vector_within hs (lv + 1ul) (V.size_of hs))))
+    //          hh0 hh3);
+    // mt_retract_to_modifies_rec_helper lv hs hh0;
+    // V.loc_vector_within_disjoint hs lv (lv + 1ul) (lv + 1ul) (V.size_of hs);
+    // V.loc_vector_within_included hs lv (lv + 1ul);
+    // RV.rv_loc_elems_included hh2 hs (lv + 1ul) (V.size_of hs);
+    // assert (loc_disjoint
+    //          (V.loc_vector_within hs lv (lv + 1ul))
+    //          (RV.rv_loc_elems hh2 hs (lv + 1ul) (V.size_of hs)));
+    // V.get_preserved hs lv
+    //   (loc_union
+    //     (RV.rv_loc_elems hh2 hs (lv + 1ul) (V.size_of hs))
+    //     (V.loc_vector_within hs (lv + 1ul) (V.size_of hs)))
+    //   hh2 hh3;
+    // assert (V.size_of (V.get hh3 hs lv) ==
+    //         j - offset_of i);
+    // assert (RV.rv_inv hh3 hs);
+    // mt_safe_elts_constr hh3 lv hs i ( j);
+    // assert (mt_safe_elts hh3 lv hs i ( j));
+
+    // // 3-1) Correctness
+    // mt_safe_elts_spec hh2 (lv + 1ul) hs (pi / 2ul) ( j / 2ul);
+    // assert (S.equal (RV.as_seq hh3 hs)
+    //                 (High.mt_retract_to_ (U32.v lv + 1) (RV.as_seq hh2 hs)
+    //                   (U32.v pi / 2) (U32.v i / 2) (U32.v ( j) / 2)));
+    // mt_safe_elts_spec hh0 lv hs pi ( j);
+    // High.mt_retract_to_rec
+    //   (U32.v lv) (RV.as_seq hh0 hs)
+    //   (U32.v pi) (U32.v i) (U32.v ( j));
+    // assert (S.equal (RV.as_seq hh3 hs)
+    //                 (High.mt_retract_to_ (U32.v lv) (RV.as_seq hh0 hs)
+    //                   (U32.v pi) (U32.v i) (U32.v ( j))))
+//  end
+#reset-options
+
+private
+inline_for_extraction
+val mt_retract_to_pre_nst: mtv:merkle_tree -> r:offset_t -> Tot bool
+let mt_retract_to_pre_nst mtv r =
+  offsets_connect (MT?.offset mtv) r &&
+  (let r = split_offset (MT?.offset mtv) r in
+   MT?.i mtv <= r && r < MT?.j mtv)
+
+val mt_retract_to_pre: mt:mt_p -> r:offset_t -> HST.ST bool
+  (requires (fun h0 -> mt_safe h0 mt))
+  (ensures (fun _ _ _ -> True))
+let mt_retract_to_pre mt r =
+  let h0 = HST.get() in
+  let mtv = !*mt in
+  mt_retract_to_pre_nst mtv r
+
+#reset-options "--z3rlimit 20 --initial_fuel 1 --max_fuel 1 --initial_ifuel 0 --max_ifuel 0"
+val mt_retract_to:
+  mt:mt_p ->
+  r:offset_t ->
+  HST.ST unit
+   (requires (fun h0 -> mt_safe h0 mt /\ mt_retract_to_pre_nst (B.get h0 mt 0) r))
+   (ensures (fun h0 _ h1 ->
+     // memory safety
+     modifies (mt_loc mt) h0 h1 /\
+     mt_safe h1 mt /\
+     // correctness
+     (let mtv = B.get h0 mt 0 in
+      let off = MT?.offset mtv in
+      let r = split_offset off r in
+      High.mt_retract_to (mt_lift h0 mt) (U32.v r) == mt_lift h1 mt)))
+
+#reset-options "--z3rlimit 100 --initial_fuel 1 --max_fuel 1 --initial_ifuel 0 --max_ifuel 0 --admit_smt_queries true"
+let rec mt_retract_to mt r =
+  let hh0 = HST.get () in
+  let mtv = !*mt in
+  let offset = MT?.offset mtv in
+  let r = split_offset offset r in
+  let hs = MT?.hs mtv in
+  mt_retract_to_ hs 0ul (MT?.i mtv) (r + 1ul) (MT?.j mtv);
+  let hh1 = HST.get () in
+  RV.rv_loc_elems_included hh0 hs 0ul (V.size_of hs);
+  V.loc_vector_within_included hs 0ul (V.size_of hs);
+  RV.rv_inv_preserved
+    (MT?.rhs mtv)
+    (loc_union
+      (RV.rv_loc_elems hh0 hs 0ul (V.size_of hs))
+      (V.loc_vector_within hs 0ul (V.size_of hs)))
+    hh0 hh1;
+  RV.as_seq_preserved
+    (MT?.rhs mtv)
+    (loc_union
+      (RV.rv_loc_elems hh0 hs 0ul (V.size_of hs))
+      (V.loc_vector_within hs 0ul (V.size_of hs)))
+    hh0 hh1;
+  Rgl?.r_sep hreg (MT?.mroot mtv)
+    (loc_union
+      (RV.rv_loc_elems hh0 hs 0ul (V.size_of hs))
+      (V.loc_vector_within hs 0ul (V.size_of hs)))
+    hh0 hh1;
+  mt *= MT (MT?.offset mtv) (r+1ul) (MT?.j mtv) hs (MT?.rhs_ok mtv) (MT?.rhs mtv) (MT?.mroot mtv);
+  let hh2 = HST.get () in
+  RV.rv_inv_preserved (MT?.hs mtv) (B.loc_buffer mt) hh1 hh2;
+  RV.rv_inv_preserved (MT?.rhs mtv) (B.loc_buffer mt) hh1 hh2;
+  RV.as_seq_preserved (MT?.hs mtv) (B.loc_buffer mt) hh1 hh2;
+  RV.as_seq_preserved (MT?.rhs mtv) (B.loc_buffer mt) hh1 hh2;
+  Rgl?.r_sep hreg (MT?.mroot mtv) (B.loc_buffer mt) hh1 hh2;
+  mt_safe_elts_preserved 0ul hs (r+1ul) (MT?.j mtv) (B.loc_buffer mt) hh1 hh2
 #reset-options
 
 /// Client-side verification
